\section*{Solution}

Given electromagnetic waves are \[\vb{E}(\vb{r},t)=\vb{E}_0\exp\qty(i\qty(\vb{k}\vdot\vb{r}-\omega{t}))\]
\[\vb{B}(\vb{r},t)=\vb{B}_0\exp\qty(i\qty(\vb{k}\vdot\vb{r}-\omega{t}))\]
\subsection*{(a)}
Wave equation \[\frac{1}{c^2}\pdv[2]{u}{t}=\laplacian{u}\qq{where}\laplacian{u}=\pdv[2]{u}{x}+\pdv[2]{u}{y}+\pdv[2]{u}{z}\]

\[\pdv{u}{x}=(ik_x)\vb{E}_0\exp\qty(i\qty(\vb{k}\vdot\vb{r}-\omega{t}))\]

\[\pdv[2]{u}{x}=(ik_x)^2\vb{E}_0\exp\qty(i\qty(\vb{k}\vdot\vb{r}-\omega{t}))\]
Similarly,
\[\pdv[2]{u}{x}=(ik_x)^2\vb{E}_0\exp\qty(i\qty(\vb{k}\vdot\vb{r}-\omega{t}))\]
\[\pdv[2]{u}{x}=(ik_x)^2\vb{E}_0\exp\qty(i\qty(\vb{k}\vdot\vb{r}-\omega{t}))\]
Hence,
\[\laplacian{u}=-(k^2_x+k^2_y+k^2_z)\vb{E}_0\exp\qty(i\qty(\vb{k}\vdot\vb{r}-\omega{t}))=-k^2\vb{E}_0\exp\qty(i\qty(\vb{k}\vdot\vb{r}-\omega{t}))\]
\[\pdv{u}{t}=(i\omega)\vb{E}_0\exp\qty(i\qty(\vb{k}\vdot\vb{r}-\omega{t}))\]
\[\pdv[2]{u}{t}=(i\omega)^2\vb{E}_0\exp\qty(i\qty(\vb{k}\vdot\vb{r}-\omega{t}))\]
Since $c^2=\frac{\omega^2}{k^2}$,
\[\pdv[2]{u}{t}=-\omega^2\vb{E}_0\exp\qty(i\qty(\vb{k}\vdot\vb{r}-\omega{t}))=-k^2c^2\vb{E}_0\exp\qty(i\qty(\vb{k}\vdot\vb{r}-\omega{t}))\]

\[\pdv[2]{u}{t}=-k^2c^2\vb{E}_0\exp\qty(i\qty(\vb{k}\vdot\vb{r}-\omega{t}))=c^2\qty(-k^2\vb{E}_0\exp\qty(i\qty(\vb{k}\vdot\vb{r}-\omega{t})))=c^2\laplacian{\vb{E}}\]
\[\frac{1}{c^2}\pdv[2]{\vb{E}}{t}=\laplacian{\vb{E}}\]
Hence $\vb{E}(\vb{r},t)=\vb{E}_0\exp\qty(i\qty(\vb{k}\vdot\vb{r}-\omega{t}))$ satisfies the wave equation.\\
Similarly $\vb{B}(\vb{r},t)=\vb{B}_0\exp\qty(i\qty(\vb{k}\vdot\vb{r}-\omega{t}))$ satisfies the wave equation.
\subsection*{(b)}
Maxwell's equations in vacuum, with no charges and currents are
\[\curl{\vb{E}}=-\frac{1}{c}\pdv{\vb{B}}{t}\quad\curl{\vb{B}}=\frac{1}{c}\pdv{\vb{E}}{t}\quad\div{\vb{E}}=0\quad\div{\vb{B}}=0\]
\subsubsection*{b.1}
\[\div{\vb{E}}=\pdv{E_x}{x}+\pdv{E_y}{y}+\pdv{E_z}{z}\]
\[\div{\vb{E}}=(ik_x)(E_{0x})\exp\qty(i\qty(\vb{k}\vdot\vb{r}-\omega{t}))+(ik_y)(E_{0y})\exp\qty(i\qty(\vb{k}\vdot\vb{r}-\omega{t}))+(ik_z)(E_{0z})\exp\qty(i\qty(\vb{k}\vdot\vb{r}-\omega{t}))\]
\[\div{\vb{E}}=i(\vb{k}\vdot{\vb{E}_0})\exp\qty(i\qty(\vb{k}\vdot\vb{r}-\omega{t}))\]
Hence $\div{\vb{E}}=0$ iff $\vb{k}\vdot\vb{E}_0=0$.\\
Similarly $\div{\vb{B}}=0$ iff $\vb{k}\vdot\vb{B}_0=0$.
\[
\curl{\vb{E}}=
\begin{vmatrix}
\vu{x}& \vu{y}& \vu{z} \\
\pdv{x}& \pdv{y}& \pdv{z} \\
E_{0x}& E_{0y}& E_{0z}
\end{vmatrix}
\]
\[=\vu{i}\qty[\pdv{E_{0z}}{y}-\pdv{E_{0y}}{z}]-\vu{j}\qty[\pdv{E_{0z}}{x}-\pdv{E_{0x}}{z}]+\vu{k}\qty[\pdv{E_{0y}}{x}-\pdv{E_{0x}}{y}]\]
\[=\qty[\vu{i}\qty[k_yE_{0z}-k_zE_{0y}]-\vu{j}\qty[k_xE_{0z}-k_zE_{0x}]+\vu{k}\qty[k_xE_{0y}-k_yE_{0x}]]\qty[\exp\qty(i\qty(\vb{k}\vdot\vb{r}-\omega{t}))](i)\]
\[=\qty(\vb{k}\cp\vb{E}_0)\exp\qty(i\qty(\vb{k}\vdot\vb{r}-\omega{t}))(i)\]
\[\pdv{\vb{B}}{t}=\qty(-i\omega)\vb{B}_0\exp\qty(i\qty(\vb{k}\vdot\vb{r}-\omega{t}))\]
\[\qq{Hence} \curl{\vb{E}}=-\frac{1}{c}\pdv{\vb{B}}{t}\qq{iff} \vb{k}\cp\vb{E}_0=\frac{\omega}{c}\vb{B}_0\]
\[\qq{Similarly} \curl{\vb{B}}=\frac{1}{c}\pdv{\vb{E}}{t}\qq{iff} \vb{k}\cp\vb{B}_0=-\frac{\omega}{c}\vb{E}_0\]
Since $\vb{k}\vdot\vb{E}_0=0$ and $\vb{k}\vdot\vb{E}_0=0$, $\vb{E}$ and $\vb{B}$ are perpendicular to $\vb{k}$.
\subsubsection*{b.2}
Define \[\vb{B}_0=\frac{c}{\omega}\qty(\vb{k}\cp\vb{E}_0)\]
Since $\vb{k}$ and $\vb{E}_0$ are perpendicular to each other, $\vb{k}\vdot\vb{E}_0=0$.
\[\vb{k}\vdot\vb{B}_0=\frac{c}{\omega}\vb{k}\vdot\qty(\vb{k}\cp\vb{E}_0)=\frac{c}{\omega}\vb{E}_0\vdot\qty(\vb{k}\cp\vb{k})=0\]
\[\vb{k}\cp\vb{B}_0=\frac{c}{\omega}\vb{k}\cp\qty(\vb{k}\cp\vb{E}_0)=\frac{c}{\omega}\qty[\vb{k}\qty(\vb{k}\vdot\vb{E}_0)-\vb{E}_0\qty(\vb{k}\vdot\vb{k})]=-k^2\frac{c}{\omega}\vb{E}_0=-\frac{\omega}{c}\vb{E}_0\]
\[\qq{Hence} \omega^2=c^2k^2\implies\omega=\pm ck\]
