% !TEX TS-program = pdflatex
% !TEX encoding = UTF-8 Unicode

\documentclass[12pt]{article}

\usepackage[utf8]{inputenc} 

\usepackage{geometry}
\geometry{a4paper} 
\geometry{margin=0.25in} 
\geometry{portrait}

\usepackage{amsmath}
\usepackage{physics}
\usepackage{tikz} 

\title{gravitation}
\author{vijayabhaskar badireddi}
%\date{} 

\begin{document}
%\maketitle
\section*{solution}
Two point masses $m_1$ and $m_2$ are located at position vectors $\vb{r}_1$ and $\vb{r}_2$.\\ The center of mass of the system is located at 
\[\vb{r}_c=\frac{m_1\vb{r}_1+m_2\vb{r}_2}{m_1+m_2}\]
Position vector of $m_1$ with respect to center of mass is $\vb{r}_{1c}=\vb{r}_1-\vb{r}_c$.
\[\vb{r}_{1c}=\vb{r}_1-\vb{r}_c=\vb{r}_1-\frac{m_1\vb{r}_1+m_2\vb{r}_2}{m_1+m_2}=\frac{m_2(\vb{r}_1-\vb{r}_2)}{m_1+m_2}\]
Position vector of $m_2$ with respect to center of mass is $\vb{r}_{2c}=\vb{r}_2-\vb{r}_c$.
\[\vb{r}_{2c}=\vb{r}_2-\vb{r}_c=\vb{r}_2-\frac{m_1\vb{r}_1+m_2\vb{r}_2}{m_1+m_2}=\frac{m_2(\vb{r}_2-\vb{r}_1)}{m_1+m_2}\]
Gravitational force on $m_1$ due to $m_2$ is given by 
\[\vb{F}_{12}=-\frac{Gm_1m_2(\vb{r}_1-\vb{r}_2)}{\vqty{\vb{r}_1-\vb{r}_2}^3}\]
Substitute for $\vb{r}_1-\vb{r}_2$ using the equation \[\vb{r}_{1c}=\frac{m_2(\vb{r}_1-\vb{r}_2)}{m_1+m_2}\implies(\vb{r}_1-\vb{r}_2)=\frac{m_1+m_2}{m_2}\vb{r}_{1c}\]
\[\vb{F}_{12}=-\frac{Gm_1m_2(\vb{r}_1-\vb{r}_2)}{\vqty{\vb{r}_1-\vb{r}_2}^3}=-\frac{Gm_1m_2(\frac{m_1+m_2}{m_2}\vb{r}_{1c})}{\vqty{\frac{m_1+m_2}{m_2}\vb{r}_{1c}}^3}=-\frac{Gm_1m_2(\vb{r}_{1c})}{\qty(\frac{m_1+m_2}{m_2})^2\vqty{\vb{r}_{1c}}^3}=-\frac{Gm_1m_2^3(\vb{r}_{1c})}{(m_1+m_2)^2\vqty{\vb{r}_{1c}}^3}\]
Gravitational force on $m_2$ due to $m_1$ is given by 
\[\vb{F}_{21}=-\frac{Gm_2m_1(\vb{r}_2-\vb{r}_1)}{\vqty{\vb{r}_2-\vb{r}_1}^3}\]
Substitute for $\vb{r}_2-\vb{r}_1$ using the equation \[\vb{r}_{2c}=\frac{m_1(\vb{r}_2-\vb{r}_1)}{m_1+m_2}\implies(\vb{r}_2-\vb{r}_1)=\frac{m_1+m_2}{m_2}\vb{r}_{2c}\]
\[\vb{F}_{21}=-\frac{Gm_2m_1(\vb{r}_2-\vb{r}_1)}{\vqty{\vb{r}_2-\vb{r}_1}^3}=-\frac{Gm_2m_1(\frac{m_1+m_2}{m_1}\vb{r}_{2c})}{\vqty{\frac{m_1+m_2}{m_1}\vb{r}_{2c}}^3}=-\frac{Gm_2m_1(\vb{r}_{2c})}{\qty(\frac{m_1+m_2}{m_1})^2\vqty{\vb{r}_{2c}}^3}=-\frac{Gm_2m_1^3(\vb{r}_{2c})}{(m_1+m_2)^2\vqty{\vb{r}_{2c}}^3}\]
Equation of motion of $m_1$ is \[m_1\dv[2]{\vb{r}_1}{t}=\vb{F}_{12}\]
Since $\vb{r}_1=\vb{r}_c+\vb{r}_{1c}$,
\[\dv[2]{\vb{r}_1}{t}=\dv[2]{\vb{r}_c}{t}+\dv[2]{\vb{r}_{1c}}{t}=0+\dv[2]{\vb{r}_{1c}}{t}\]
Since net external force on the system is zero, center of mass does not move.Hence $\vb{r}_c$ is constant and $\dv[2]{\vb{r}_c}{t}=0$.\\
Equation of motion of $m_1$ is \[m_1\dv[2]{\vb{r}_1}{t}=m_1\dv[2]{\vb{r}_{1c}}{t}=\vb{F}_{12}=-\frac{Gm_1m_2^3(\vb{r}_{1c})}{(m_1+m_2)^2\vqty{\vb{r}_{1c}}^3}\]
Similarly equation of motion of $m_2$ is \[m_2\dv[2]{\vb{r}_2}{t}=m_2\dv[2]{\vb{r}_{2c}}{t}=\vb{F}_{21}=-\frac{Gm_2m_1^3(\vb{r}_{2c})}{(m_1+m_2)^2\vqty{\vb{r}_{2c}}^3}\]
\[\boxed{m_1\dv[2]{\vb{r}_{1c}}{t}=-\frac{Gm_1m_2^3(\vb{r}_{1c})}{(m_1+m_2)^2\vqty{\vb{r}_{1c}}^3}}\]
\[\boxed{m_2\dv[2]{\vb{r}_{2c}}{t}=-\frac{Gm_2m_1^3(\vb{r}_{2c})}{(m_1+m_2)^2\vqty{\vb{r}_{2c}}^3}}\]
\section*{reaching the sun}
\subsection*{Orbital Period}
\[\frac{mV^2}{R}=\frac{GMm}{R^2}\]
Orbital velocity is \[V=\sqrt{\frac{GM}{R}}\]
Time period is 
\[T=2\pi\sqrt{\frac{R^3}{GM}}\]
Now an object is released with zero velocity at a distance $R$ from sun. Force on the object is \[\vec{F}=-\frac{GMm}{r^2}\hat{r}\]
\[m\dv{V}{t}=-\frac{GMm}{r^2}\]
\[V\pdv{V}{r}=-\frac{GM}{r^2}\]
\[\int_0^VV\dd{V}=GM\int_R^r-\frac{\dd{r}}{r^2}\]
\[\frac{V^2}{2}=GM\left(\frac{1}{r}-\frac{1}{R}\right)\]
\[V=-\sqrt{2GM}\left(\frac{R-r}{Rr}\right)^{1/2}\]
\[\dv{r}{t}=-\sqrt{2GM}\left(\frac{R-r}{Rr}\right)^{1/2}\]
\[\left(\frac{Rr}{R-r}\right)^{1/2}\dd{r}=-\sqrt{2GM}\dd{t}\]
\[-\int^0_R\left(\frac{Rr}{R-r}\right)^{1/2}\dd{r}=\sqrt{2GM}\int_0^{T'}\dd{t}\]
Substitute $r=R\sin^2\theta$ and $\dd{r}=2R\sin\theta\cos\theta\dd{\theta}$
\[\sqrt{2GM}\,T'=-\int_R^0\left(\frac{Rr}{R-r}\right)^{1/2}\dd{r}\]
\[\sqrt{2GM}\,T'=-\int_{\pi/2}^0\left[\frac{R^2\sin^2\theta}{R(1-\sin^2\theta)}\right]^{1/2}2R\sin\theta\cos\theta\dd{\theta}\]
\[\sqrt{2GM}\,T'=-\int_{\pi/2}^02R^{3/2}\sin^2\theta\dd{\theta}=2R^{3/2}\int_0^{\pi/2}\left[\frac{1-\sin2\theta}{2}\right]\dd{\theta}\]
\[\sqrt{2GM}\,T'=\frac{\pi R^{3/2}}{2}\]
\[T'=\frac{1}{4\sqrt{2}}\left[2\pi\sqrt{\frac{R^3}{GM}}\right]=\frac{T}{4\sqrt{2}}\]
\end{document}
