\section*{harmonicoscillator}

\[\hat{H}\psi=E\psi\]
\[-\frac{\hbar^2}{2m}\dv[2]{\psi}{x}+V(x)\psi=E\psi\]
Since the potential is $V(s)=\frac{1}{2}kx^2=\frac{1}{2}m\omega^2x^2$
\[-\frac{\hbar^2}{2m}\dv[2]{\psi}{x}+\frac{1}{2}m\omega^2x^2\psi=E\psi\]
\[\dv[2]{\psi}{x}-\frac{m^2\omega^2}{\hbar^2}x^2\psi=-\frac{2Em}{\hbar^2}\psi\]
Redefine $z=\sqrt{\frac{m\omega}{\hbar}}x$.
\[\dv[2]{\psi}{x}=\frac{m\omega}{\hbar}\dv[2]{\psi}{z}\]
\[\frac{m\omega}{\hbar}\dv[2]{\psi}{z}-\frac{m\omega}{\hbar}z^2\psi=-\frac{2Em}{\hbar^2}\psi\]
\[\dv[2]{\psi}{z}-z^2\psi=-\frac{\hbar}{m\omega}\frac{2Em}{\hbar^2}\psi=-\frac{2E}{\hbar\omega}\psi\]
\[\dv[2]{\psi}{z}+\qty(\frac{2E}{\hbar\omega}-z^2)\psi=0\]
Substitute $\psi=H(\zeta)e^{-z^2/2}$	
\subsection*{5.9}
\[\mel{x}{n}{k}=\]
