\section*{randt}
Wave is coming in from $-\infty$ towards right. Particles have energy $\frac{V_0}{2}<E<V_0$.\\
Potential is 
$$
V(x)=
\begin{cases}
0 \qq{for} -\infty < x \le -a \\
V_0 \qq{for} |x|<a\\
\frac{V_0}{2} \qq{for} x\ge a
\end{cases}
$$
Schrodinger equation is
\[-\frac{\hbar^2}{2m}\dv[2]{\psi}{x}+V(x)\psi=E\psi\]
For region $1$, $V(x)=0$\\
\[\psi_1''=\frac{2mE}{\hbar^2}\psi_1=0\Rightarrow\psi_1''+k_1^2\psi_1=0\qq{where}k_1=\sqrt{\frac{2mE}{\hbar^2}}\]
Solution is 
\[\psi_1=A_1e^{ik_1x}+B_1e^{-ik_1x}\]
The term $e^{ik_1x}$ represents a wave coming from $-\infty$ to right.\\
The term $e^{-ik_1x}$ represents a wave coming from $\infty$ to left.\\
For region $2$, $V(x)=V_0$\\
\[\psi_2''+\frac{2m(E-v_0)}{\hbar^2}\psi_2=0\Rightarrow\psi_2''-k_2^2\psi_2=0\qq{where}k_2=\sqrt{\frac{2m(V_0-E)}{\hbar^2}}\]
Solution is 
\[\psi_2=A_2e^{k_2x}+B_2e^{-k_2x}\]
For region $3$, $V(x)=\frac{V_0}{2}$\\
\[\psi_3''+\frac{2m(E-v_0/2)}{\hbar^2}\psi_3=0\Rightarrow\psi_3''+k_3^2\psi_3=0\qq{where}k_3=\sqrt{\frac{2m(E-V_0/2)}{\hbar^2}}\]
Solution is 
\[\psi_3=A_3e^{ik_3x}+B_3e^{-ik_3x}\]
In region $3$, there will be no wave coming from $+\infty$ to the left. Hence $B_3=0$.\\
Since wave function is continuous at $x=-a$ and $x=a$,
\[\psi_1(x=-a)=\psi_2(x=-a)\qq{and}\psi_2(x=+a)=\psi_3(x=+a)\]
\[A_1e^{-ik_1a}+B_1e^{ik_1a}=A_2e^{-k_2a}+B_2e^{k_2a}\tag{1}\]
\[A_2e^{k_2a}+B_2e^{-k_2a}=A_3e^{ik_3a}\tag{2}\]
Since the derivative of the wave function is continuous at $x=-a$ and $x=a$,
\[\psi_1'(x=-a)=\psi_2'(x=-a)\qq{and}\psi_2'(x=+a)=\psi_3'(x=+a)\]
\[ik_1A_1e^{-ik_1a}-ik_1B_1e^{ik_1a}=k_2A_2e^{-k_2a}-k_2B_2e^{k_2a}\tag{3}\]
\[k_2A_2e^{k_2a}-k_2B_2e^{-k_2a}=ik_3A_3e^{ik_3a}\tag{4}\]
Using equations $(2)$ and $(4)$,
\[A_2e^{k_2a}=\frac{1}{2}\qty[1+\frac{ik_3}{k_2}]B_3e^{ik_3a}\]
\[A_2=\qty[\frac{k_2+ik_3}{2k_2}]B_3e^{(ik_3-k_2)a}\]
\[B_2e^{-k_2a}=\frac{1}{2}\qty[1-\frac{ik_3}{k_2}]B_3e^{ik_3a}\]
\[B_2=\qty[\frac{k_2-ik_3}{2k_2}]B_3e^{(ik_3+k_2)a}\]
\newpage
Using equations $(1)$ and $(3)$,
\[A_1e^{-ik_1a}=\frac{1}{2}\qty[\qty(1+\frac{k_2}{ik_1})A_2e^{-k_2a}+\qty(1-\frac{k_2}{ik_1})B_2e^{k_2a}]\]
\[A_1=\qty(\frac{k_2+ik_1}{2ik_1})A_2e^{-(k_2-ik_1)a}-\qty(\frac{k_2-ik_1}{2ik_1})B_2e^{(k_2+ik_1)a}\]
\[B_1e^{ik_1a}=\frac{1}{2}\qty[\qty(1-\frac{k_2}{ik_1})A_2e^{-k_2a}+\qty(1+\frac{k_2}{ik_1})B_2e^{k_2a}]\]
\[B_1=-\qty(\frac{k_2-ik_1}{2ik_1})A_2e^{-(k_2+ik_1)a}+\qty(\frac{k_2+ik_1}{2ik_1})B_2e^{(k_2-ik_1)a}\]
Substituting the expressions for $A_2$ and $B_2$,

\[A_1=\qty(\frac{k_2+ik_1}{2ik_1})\qty(\frac{k_2+ik_3}{2k_2})B_3e^{(ik_3-k_2)a}e^{-(k_2-ik_1)a}-\qty(\frac{k_2-ik_1}{2ik_1})\qty(\frac{k_2-ik_3}{2k_2})B_3e^{(ik_3+k_2)a}e^{(k_2+ik_1)a}\]
\[A_1=B_3e^{i(k_1+k_3)a}\qty[\qty(\frac{k_2+ik_1}{2ik_1})\qty(\frac{k_2+ik_3}{2k_2})e^{-2k_2a}-\qty(\frac{k_2-ik_1}{2ik_1})\qty(\frac{k_2-ik_3}{2k_2})e^{2k_2a}]\]
\[A_1^*=B_3^*e^{-i(k_1+k_3)a}\qty[\qty(\frac{k_2+ik_1}{2ik_1})\qty(\frac{k_2+ik_3}{2k_2})e^{2k_2a}-\qty(\frac{k_2-ik_1}{2ik_1})\qty(\frac{k_2-ik_3}{2k_2})e^{-2k_2a}]\]
\[|A_1|^2=|B_3|^2\qty[\qty(\frac{k_2+ik_1}{2ik_1})^2\qty(\frac{k_2+ik_3}{2k_2})^2+\qty(\frac{k_2-ik_1}{2ik_1})^2\qty(\frac{k_2-ik_3}{2k_2})^2+\qty(\frac{k_2^2+k_1^2}{4k_1^2})\qty(\frac{k_2^2+k_3^2}{4k_2^2})2\cosh{4k_2a}]\]
\[|A_1|^2=|B_3|^2\qty[\qty(\frac{(k_2^2+k_1^2)(k_2^2+k_3^2)}{16k_1^2k_2^2})2\cosh{4k_2a}-\qty[\frac{(k_2+ik_1)^2(k_2+ik_3)^2+(k_2-ik_1)^2(k_2-ik_3)^2}{16k_1^2k_2^2}]]\]
\[|A_1|^2=2|B_3|^2\qty[\qty(\frac{(k_2^2+k_1^2)(k_2^2+k_3^2)}{16k_1^2k_2^2})\cosh{4k_2a}-\qty(\frac{(k_2^2+k_1^2)(k_2^2+k_3^2)-4k_1k_2^2k_3}{16k_1^2k_2^2})]\]
